deps/poulet4/lib/P4automata/Benchmarks/IPOptionsProofSmall.v
@@ -1,0 +1,164 @@
+Require Import Poulet4.P4automata.Benchmarks.ProofHeader.
+Require Import Poulet4.P4automata.Benchmarks.IPOptions.
+
+
+Declare ML Module "mirrorsolve".
+
+Ltac hashcons_list xs :=
+  match xs with
+  | ?x :: ?xs =>
+    hashcons_list xs;
+    let v := fresh "v" in 
+    set (v := x)
+    
+  | ?x :: nil =>
+    let v := fresh "v" in 
+    set (v := x)
+  | nil =>
+    idtac
+  end.
+
+Module SelfComparison.
+    
+  Notation H := (IPOptions32.header + IPOptions32.header).
+  Notation A := (Sum.sum IPOptions32.aut IPOptions32.aut).
+  Notation conf := (P4automaton.configuration (P4A.interp A)).
+
+
+  Definition r_states :=
+    Eval vm_compute in (Reachability.reachable_states
+                          A
+                          10
+                          IPOptions32.Parse0
+                          IPOptions32.Parse0).
+
+  (* Definition r_with_len := Eval vm_compute in (length r_states, r_states).
+
+  Print r_with_len. *)
+
+  Definition top : Relations.rel conf := fun _ _ => True.
+  Definition top' : Relations.rel (state_template A) := fun _ _ => True.
+
+  ClearEnvCtors.
+
+  RegisterEnvCtors
+    (IPOptions32.Scratch8, FirstOrderConfRelSimplified.Bits 8)
+    (  IPOptions32.Scratch16, FirstOrderConfRelSimplified.Bits 16)
+    (  IPOptions32.T0, FirstOrderConfRelSimplified.Bits 8)
+    (  IPOptions32.L0, FirstOrderConfRelSimplified.Bits 8)
+    (  IPOptions32.V0, FirstOrderConfRelSimplified.Bits 24)
+    (  IPOptions32.T1, FirstOrderConfRelSimplified.Bits 8)
+    (  IPOptions32.L1, FirstOrderConfRelSimplified.Bits 8)
+    (  IPOptions32.V1, FirstOrderConfRelSimplified.Bits 24).
+
+  Inductive mark : nat -> Type := M : forall (n: nat), mark n.
+    
+  Ltac measure_goals := match goal with 
+    | |- pre_bisimulation _ _ _ _ ?R _ _ => 
+      let x := fresh "rem_goals" in
+      pose proof (x := M (length R));
+      vm_compute in x;
+      match goal with 
+      | H : mark ?n |- _ => 
+        idtac "remaining goals: " n;
+        clear H
+      end
+    end.
+
+  Lemma prebisim_babyip:
+    forall q1 q2,
+      interp_conf_rel' {| cr_st := {|
+                          cs_st1 := {|
+                            st_state := inl (inl (IPOptions32.Parse0));
+                            st_buf_len := 0;
+                          |};
+                          cs_st2 := {|
+                            st_state := inl (inr (IPOptions32.Parse0));
+                            st_buf_len := 0;
+                          |};
+                        |};
+                        cr_ctx := BCEmp;
+                        cr_rel := btrue;
+                    |} q1 q2 ->
+    pre_bisimulation A
+                    (wp r_states)
+                    top
+                    []
+                    (mk_init _ _ _ A 10 IPOptions32.Parse0 IPOptions32.Parse0)
+                    q1 q2.
+  Proof.
+    idtac "running ipoptions ref self-comparison bisimulation".
+
+    intros.
+    set (rel0 := (mk_init _ _ _ A 10 IPOptions32.Parse0 IPOptions32.Parse0)).
+    vm_compute in rel0.
+    subst rel0.
+    clear H.
+
+    Set Ltac Profiling.
+
+    (* match goal with 
+    | |- pre_bisimulation _ _ _ _ ?G _ _ =>
+      hashcons_list G
+    end. *)
+
+    (* Set Ltac Profiling. *)
+
+
+
+    do 25 ((time "single step" run_bisim top top' r_states);
+    match goal with 
+    | |- pre_bisimulation _ _ _ (?N :: _) _ _ _  => 
+      let r := fresh "r" in 
+      set (r := N)
+    | _ => idtac
+    end).
+
+    do 25 ((time "single step" run_bisim top top' r_states);
+    match goal with 
+    | |- pre_bisimulation _ _ _ (?N :: _) _ _ _  => 
+      let r := fresh "r" in 
+      set (r := N)
+    | _ => idtac
+    end).
+
+    do 25 ((time "single step" run_bisim top top' r_states);
+    match goal with 
+    | |- pre_bisimulation _ _ _ (?N :: _) _ _ _  => 
+      let r := fresh "r" in 
+      set (r := N)
+    | _ => idtac
+    end).
+
+    do 25 ((time "single step" run_bisim top top' r_states);
+    match goal with 
+    | |- pre_bisimulation _ _ _ (?N :: _) _ _ _  => 
+      let r := fresh "r" in 
+      set (r := N)
+    | _ => idtac
+    end).
+
+    do 25 ((time "single step" run_bisim top top' r_states);
+    match goal with 
+    | |- pre_bisimulation _ _ _ (?N :: _) _ _ _  => 
+      let r := fresh "r" in 
+      set (r := N)
+    | _ => idtac
+    end).
+
+    do 25 ((time "single step" run_bisim top top' r_states);
+    match goal with 
+    | |- pre_bisimulation _ _ _ (?N :: _) _ _ _  => 
+      let r := fresh "r" in 
+      set (r := N)
+    | _ => idtac
+    end).
+
+    idtac "150 steps..., quitting...".
+
+    Show Ltac Profile.
+
+ Time Admitted.
+
+End SelfComparison.
+
